Axiomatizing ink contract deps

coq_translation/examples/ink/flipper/Crate.v
@@ -3,9 +3,129 @@ Require Import CoqOfRust.CoqOfRust.
 
 Import std.prelude.rust_2021.
 
-(* source code https://github.com/paritytech/ink/blob/master/integration-tests/flipper/lib.rs *)
+(** Axiomatization of ink deps *)
 
+(* @TODO Double check this in [CoqOfRust] *)
+Parameter usize : Set.
+
+Module Root.
+  Module ink.
+    Module storage.
+      Module traits.
+        Module AutoStorableHint.
+          Parameter Type_ : Set.
+        End AutoStorableHint.
+      End traits.
+    End storage.
+
+    Module env.
+      Parameter DefaultEnvironment : Set.
+
+      Module ContractEnv.
+        Class Trait (Self : Set) : Set := {
+            (* ??? *)
+          }.
+        
+        Parameter Env : Set.
+      End ContractEnv.
+      Module Environment.
+        Parameter AccountId : Set.
+        Parameter Balance : Set.
+        Parameter Hash : Set.
+        Parameter Timestamp : Set.
+        Parameter BlockNumber : Set.
+        Parameter ChainExtension : Set.
+        Parameter MAX_EVENT_TOPICS : usize.
+      End Environment.
+    End env.
+    Module reflect.
+      Module ConstructorOutput.
+        Parameter Error : Set.
+        (* @TODO Not sure about this, it is a guess *)
+        Parameter IS_RESULT : unit -> bool.
+      End ConstructorOutput.
+
+      Module DispatchableConstructorInfo.
+        Class Trait (Self : Set) (a b : Set) : Set := {
+          IS_RESULT : unit -> unit -> bool;
+          CALLABLE : unit -> a -> b;
+          PAYABLE : unit -> bool;
+          SELECTOR : unit -> list Z;
+          LABEL : unit -> string;
+        }.
+      End DispatchableConstructorInfo.
+
+      Module DispatchableMessageInfo.
+     (* : unit -> ImplFlipper.Self -> unit -> bool *)
+        Class Trait Self (a b : Set) := {
+            CALLABLE : unit -> Self -> a -> b;
+            MUTATES : unit -> bool;
+            PAYABLE : unit -> bool;
+            SELECTOR : unit -> list Z;
+            LABEL : unit -> string;
+          }.
+      End DispatchableMessageInfo.
+    End reflect.
+    Module codegen.
+      Module ContractCallBuilder.
+        Parameter Type_ : Set.
+      End ContractCallBuilder.
+    End codegen.
+  End ink.
+End Root.
+
+(* source code https://github.com/paritytech/ink/blob/master/integration-tests/flipper/lib.rs *)
 Module flipper.
+
+  (* I had to move this up *)
+  Module Flipper.
+    Record t : Set := {
+      value : Root.ink.storage.traits.AutoStorableHint.Type_;
+        (* I have to put _ after Type because Type is reserved in Coq *)
+    }.
+    
+    Global Instance Get_value : Notation.Dot "value" := {
+      Notation.dot '(Build_t x0) := x0;
+    }.
+  End Flipper.
+  Definition Flipper : Set := Flipper.t.
+
+  Module ImplFlipper.
+    Definition Self := Flipper.
+
+    (* @TODO added by hand *)
+    Definition new (x : Root.ink.storage.traits.AutoStorableHint.Type_) : Self := Flipper.Build_t x.
+
+    (* @TODO added by hand *)
+    Parameter new_default : unit -> Flipper.
+
+    (* @TODO added by hand *)
+    Parameter flip : Self -> Self.
+
+    (* @TODO added by hand *)
+    Parameter get : Self -> bool.
+    
+    (* @TODO added by hand *)
+    Global Instance AssociatedFunction_new : Notation.DoubleColon Self "new" := {
+      Notation.double_colon := new;
+    }.
+
+    (* @TODO added by hand *)
+    Global Instance AssociatedFunction_new_default : Notation.DoubleColon Self "new_default" := {
+      Notation.double_colon := new_default;
+    }.
+
+    (* @TODO added by hand *)
+    Global Instance AssociatedFunction_flip : Notation.DoubleColon Self "flip" := {
+      Notation.double_colon := flip;
+    }.
+
+    (* @TODO added by hand *)
+    Global Instance AssociatedFunction_get : Notation.DoubleColon Self "get" := {
+      Notation.double_colon := get;
+    }.
+  End ImplFlipper.
+
   Module Impl_Root_ink_env_ContractEnv_for_Flipper.
     Definition Self := Flipper.
     
@@ -32,18 +152,11 @@ Module flipper.
   Definition MAX_EVENT_TOPICS : usize :=
     Root.ink.env.Environment.MAX_EVENT_TOPICS.
   
+  (* @TODO I don't know from where this came from in the translation
+     commenting it fow now *)
+  (*
   Definition _ : unit := tt.
-  
-  Module Flipper.
-    Record t : Set := {
-      value : Root.ink.storage.traits.AutoStorableHint.Type;
-    }.
-    
-    Global Instance Get_value : Notation.Dot "value" := {
-      Notation.dot '(Build_t x0) := x0;
-    }.
-  End Flipper.
-  Definition Flipper : Set := Flipper.t.
+
   
   Definition _ : unit := tt.
   
@@ -60,6 +173,7 @@ Module flipper.
   Definition _ : unit := tt.
   
   Definition _ : unit := tt.
+   *)
   
   Module Impl_Root_ink_reflect_DispatchableConstructorInfo_for_Flipper.
     Definition Self := Flipper.
@@ -78,8 +192,8 @@ Module flipper.
     Global Instance AssociatedFunction_IS_RESULT :
       Notation.DoubleColon Self "IS_RESULT" := {
       Notation.double_colon := IS_RESULT;
-    }.
-    
+      }.
+
     Definition CALLABLE (_ : unit) :=
       fun __ink_binding_0 => Flipper::["new"] __ink_binding_0.
     
@@ -112,7 +226,7 @@ Module flipper.
     Global Instance I
         :
         Root.ink.reflect.DispatchableConstructorInfo.Trait
-        Self :=
+        Self Root.ink.storage.traits.AutoStorableHint.Type_ ImplFlipper.Self :=
       {
       Root.ink.reflect.DispatchableConstructorInfo.IS_RESULT := IS_RESULT;
       Root.ink.reflect.DispatchableConstructorInfo.CALLABLE := CALLABLE;
@@ -120,12 +234,16 @@ Module flipper.
       Root.ink.reflect.DispatchableConstructorInfo.SELECTOR := SELECTOR;
       Root.ink.reflect.DispatchableConstructorInfo.LABEL := LABEL;
     }.
+    
+
   End Impl_Root_ink_reflect_DispatchableConstructorInfo_for_Flipper.
-  
-  Module Impl_Root_ink_reflect_DispatchableConstructorInfo_for_Flipper.
+
+  (* @TODO There is already a module with this same name above, so I added _2
+     to this one. *)
+  Module Impl_Root_ink_reflect_DispatchableConstructorInfo_for_Flipper_2.
     Definition Self := Flipper.
     
-    Definition Input : Set := unit.
+    Definition Input : Set := unit. (* In the previous module this was bool instaed of unit *)
     
     Definition Output : Set := Self.
     
@@ -141,7 +259,8 @@ Module flipper.
       Notation.double_colon := IS_RESULT;
     }.
     
-    Definition CALLABLE (_ : unit) := fun _ => Flipper::["new_default"] tt.
+    (* @TODO Coq fails to infer the type of the lambda parameter [_] *)
+    Definition CALLABLE (_ : unit) := fun _ : Root.ink.storage.traits.AutoStorableHint.Type_ => Flipper::["new_default"] tt.
     
     Global Instance AssociatedFunction_CALLABLE :
       Notation.DoubleColon Self "CALLABLE" := {
@@ -172,7 +291,7 @@ Module flipper.
     Global Instance I
         :
         Root.ink.reflect.DispatchableConstructorInfo.Trait
-        Self :=
+        Self Root.ink.storage.traits.AutoStorableHint.Type_ Flipper :=
       {
       Root.ink.reflect.DispatchableConstructorInfo.IS_RESULT := IS_RESULT;
       Root.ink.reflect.DispatchableConstructorInfo.CALLABLE := CALLABLE;
@@ -180,8 +299,8 @@ Module flipper.
       Root.ink.reflect.DispatchableConstructorInfo.SELECTOR := SELECTOR;
       Root.ink.reflect.DispatchableConstructorInfo.LABEL := LABEL;
     }.
-  End Impl_Root_ink_reflect_DispatchableConstructorInfo_for_Flipper.
-  
+  End Impl_Root_ink_reflect_DispatchableConstructorInfo_for_Flipper_2.
+
   Module Impl_Root_ink_reflect_DispatchableMessageInfo_for_Flipper.
     Definition Self := Flipper.
     
@@ -192,7 +311,8 @@ Module flipper.
     Definition Storage : Set := Flipper.
     
     Definition CALLABLE (_ : unit) :=
-      fun storage _ => Flipper::["flip"] storage.
+      fun storage (_ : (* @TODO added by hand, it is a guess *)Root.ink.storage.traits.AutoStorableHint.Type_) =>
+        Flipper::["flip"] storage.
     
     Global Instance AssociatedFunction_CALLABLE :
       Notation.DoubleColon Self "CALLABLE" := {
@@ -227,7 +347,14 @@ Module flipper.
       Notation.double_colon := LABEL;
     }.
     
-    Global Instance I : Root.ink.reflect.DispatchableMessageInfo.Trait Self := {
+(* unit -> ImplFlipper.Self -> Root.ink.storage.traits.AutoStorableHint.Type_ -> ImplFlipper.Self *)
+(* unit -> ImplFlipper.Self -> unit ->                                           bool *)
+
+     (* : unit -> bool *)
+     (* : unit -> bool *)
+
+    Global Instance I : Root.ink.reflect.DispatchableMessageInfo.Trait
+      Self Root.ink.storage.traits.AutoStorableHint.Type_ ImplFlipper.Self := {
       Root.ink.reflect.DispatchableMessageInfo.CALLABLE := CALLABLE;
       Root.ink.reflect.DispatchableMessageInfo.MUTATES := MUTATES;
       Root.ink.reflect.DispatchableMessageInfo.PAYABLE := PAYABLE;
@@ -235,8 +362,8 @@ Module flipper.
       Root.ink.reflect.DispatchableMessageInfo.LABEL := LABEL;
     }.
   End Impl_Root_ink_reflect_DispatchableMessageInfo_for_Flipper.
-  
-  Module Impl_Root_ink_reflect_DispatchableMessageInfo_for_Flipper.
+
+  Module Impl_Root_ink_reflect_DispatchableMessageInfo_for_Flipper_2. (* Had to add _2 here *)
     Definition Self := Flipper.
     
     Definition Input : Set := unit.
@@ -245,7 +372,7 @@ Module flipper.
     
     Definition Storage : Set := Flipper.
     
-    Definition CALLABLE (_ : unit) := fun storage _ => Flipper::["get"] storage.
+    Definition CALLABLE (_ : unit) := fun storage (_ : unit) => Flipper::["get"] storage.
     
     Global Instance AssociatedFunction_CALLABLE :
       Notation.DoubleColon Self "CALLABLE" := {
@@ -280,26 +407,26 @@ Module flipper.
       Notation.double_colon := LABEL;
     }.
     
-    Global Instance I : Root.ink.reflect.DispatchableMessageInfo.Trait Self := {
+    Global Instance I : Root.ink.reflect.DispatchableMessageInfo.Trait Self unit bool := {
       Root.ink.reflect.DispatchableMessageInfo.CALLABLE := CALLABLE;
       Root.ink.reflect.DispatchableMessageInfo.MUTATES := MUTATES;
       Root.ink.reflect.DispatchableMessageInfo.PAYABLE := PAYABLE;
       Root.ink.reflect.DispatchableMessageInfo.SELECTOR := SELECTOR;
       Root.ink.reflect.DispatchableMessageInfo.LABEL := LABEL;
     }.
-  End Impl_Root_ink_reflect_DispatchableMessageInfo_for_Flipper.
+  End Impl_Root_ink_reflect_DispatchableMessageInfo_for_Flipper_2.
   
-  Definition _ : unit := tt.
+  (* Definition _ : unit := tt. *)
   
-  Definition _ : unit := tt.
+  (* Definition _ : unit := tt. *)
   
-  Definition _ : unit := tt.
+  (* Definition _ : unit := tt. *)
   
-  Definition _ : unit := tt.
-  
+  (* Definition _ : unit := tt. *)
+
   Module FlipperRef.
     Record t : Set := {
-      inner : Root.ink.codegen.ContractCallBuilder.Type;
+      inner : Root.ink.codegen.ContractCallBuilder.Type_;
     }.
     
     Global Instance Get_inner : Notation.Dot "inner" := {
@@ -308,8 +435,41 @@ Module flipper.
   End FlipperRef.
   Definition FlipperRef : Set := FlipperRef.t.
   
+  (* @TODO example for impl Debug, remove it later *)
+  Module Impl__crate_fmt_Debug_for_Unit.
+    Definition Self := unit.
+
+    Definition fmt
+        (self : ref Self)
+        (f : mut_ref _crate.fmt.Formatter)
+        : _crate.fmt.Result :=
+      _crate.fmt.Formatter::["write_str"] f "Unit".
+
+    Global Instance Method_fmt : Notation.Dot "fmt" := {
+      Notation.dot := fmt;
+    }.
+
+    Global Instance I : _crate.fmt.Debug.Trait Self := {
+      _crate.fmt.Debug.fmt := fmt;
+    }.
+  End Impl__crate_fmt_Debug_for_Unit.
+
   Module Impl__crate_fmt_Debug_for_FlipperRef.
     Definition Self := FlipperRef.
+
+    (* @TODO added by hand *)
+    Parameter debug_struct_field1_finish :
+      mut_ref _crate.fmt.Formatter
+      -> String
+      -> String
+      -> Root.ink.codegen.ContractCallBuilder.Type_
+      -> _crate.fmt.Result.
+
+    (* @TODO added by hand *)
+    Global Instance AssociatedFunction_debug_struct_fields1_finish_method  :
+      Notation.DoubleColon _crate.fmt.Formatter "debug_struct_field1_finish" := {
+        Notation.double_colon := debug_struct_field1_finish;
+      }.
     
     Definition fmt
         (self : ref Self)
@@ -330,20 +490,45 @@ Module flipper.
     }.
   End Impl__crate_fmt_Debug_for_FlipperRef.
   
-  Definition _ : unit := tt.
+  (* Definition _ : unit := tt. *)
   
-  Definition _ : unit := tt.
+  (* Definition _ : unit := tt. *)
   
   Module Impl__crate_hash_Hash_for_FlipperRef.
     Definition Self := FlipperRef.
-    
-    Definition hash (self : ref Self) (state : mut_ref __H) : unit :=
-      _crate.hash.Hash.hash self.["inner"] state.
+
+    (* I'm very confused here *)
+
+    Parameter __H : Set.        (* ??? added by hand, was missing below *)
+
+    (* @TODO added by hand *)
+    Module _crate.
+      Module hash.
+        Module Hash.
+          (* @TODO fix these parameters, they must be generic *)
+          (* Parameter hash_ : Root.ink.codegen.ContractCallBuilder.Type_ -> mut_ref __H -> unit. *)
+
+          Class Trait (Self : Set) : Set := {
+              hash : Root.ink.codegen.ContractCallBuilder.Type_ -> mut_ref __H -> unit
+            }.
+        End Hash.
+      End hash.
+    End _crate.
+
+    (* I think this must call _crate.hash.Hash.hash
+       which is a type class function in _crate.hash.Hash.Trait *)
+    (* but I have 
+       - ?Trait: Cannot infer the implicit parameter Trait of _crate.hash.Hash.hash whose type is
+         "_crate.hash.Hash.Trait ?Self" (no type class instance found) in *)
+    Definition hash (*_ added by hand *) (self : ref Self) (state : mut_ref __H) : unit :=
+      _crate.hash.Hash.hash (Self := Self) self.["inner"] state.
     
     Global Instance Method_hash : Notation.Dot "hash" := {
       Notation.dot := hash;
     }.
     
+    (* It seems that I need this instance? in hash definition above??
+      (line 523) *)
     Global Instance I : _crate.hash.Hash.Trait Self := {
       _crate.hash.Hash.hash := hash;
     }.
